src/Lean/Elab/Tactic/BVDecide/LRAT/Actions.lean
@@ -7,9 +7,10 @@ prelude
 import Std.Sat.CNF
 
 /-!
-This module contains the definition of the LRAT format as a type `Action`, that is polymorphic over
-the variables used in the CNF. The type `IntAction := Action (Array Int) Nat` is the version that is
-used by the checker as input and should be considered the parsing target for LRAT proofs.
+This module contains the definition of the LRAT format (https://www.cs.utexas.edu/~marijn/publications/lrat.pdf)
+as a type `Action`, that is polymorphic over the variables used in the CNF. The type
+`IntAction := Action (Array Int) Nat` is the version that is used by the checker as input and should
+be considered the parsing target for LRAT proofs.
 -/
 
 namespace Lean.Elab.Tactic.BVDecide
@@ -18,7 +19,7 @@ namespace LRAT
 open Std.Sat
 
 /-- `β` is for the type of a clause, `α` is for the type of variables -/
-inductive Action (β : (Type v)) (α : (Type w))
+inductive Action (β : Type u) (α : Type v)
   | addEmpty (id : Nat) (rupHints : Array Nat)
   | addRup (id : Nat) (c : β) (rupHints : Array Nat)
   | addRat (id : Nat) (c : β) (pivot : Literal α) (rupHints : Array Nat) (ratHints : Array (Nat × Array (Nat)))
